cleaning up the chacha and salsa impl files

code/salsa-family/Hacl.Impl.Chacha20.fst
@@ -28,11 +28,10 @@ private inline_for_extraction let op_Less_Less_Less (a:h32) (s:u32{U32.v s <= 32
   (a <<^ s) |^ (a >>^ (FStar.UInt32.(32ul -^ s)))
 
 
-#reset-options "--initial_fuel 0 --max_fuel 0 --z3rlimit 100"
-
-#reset-options "--initial_fuel 0 --max_fuel 0 --initial_ifuel 0 --max_ifuel 0 --z3rlimit 100"
+#reset-options "--max_fuel 0 --z3rlimit 100"
 
 [@ "substitute"]
+private
 val constant_setup_:
   c:Buffer.buffer H32.t{length c = 4} ->
   Stack unit
@@ -52,6 +51,7 @@ let constant_setup_ st =
 
 
 [@ "substitute"]
+private
 val constant_setup:
   c:Buffer.buffer H32.t{length c = 4} ->
   Stack unit
@@ -71,6 +71,7 @@ let constant_setup st =
 
 
 [@ "substitute"]
+private
 val keysetup:
   st:Buffer.buffer H32.t{length st = 8} ->
   k:uint8_p{length k = 32 /\ disjoint st k} ->
@@ -86,6 +87,7 @@ let keysetup st k =
 
 
 [@ "substitute"]
+private
 val ivsetup:
   st:buffer H32.t{length st = 3} ->
   iv:uint8_p{length iv = 12 /\ disjoint st iv} ->
@@ -102,6 +104,7 @@ let ivsetup st iv =
 
 
 [@ "substitute"]
+private
 val ctrsetup:
   st:buffer H32.t{length st = 1} ->
   ctr:U32.t ->
@@ -176,6 +179,7 @@ let setup st k n c =
 let idx = a:U32.t{U32.v a < 16}
 
 [@ "substitute"]
+private
 val line:
   st:state ->
   a:idx -> b:idx -> d:idx -> s:U32.t{U32.v s < 32} ->
@@ -195,6 +199,7 @@ let line st a b d s =
 
 
 [@ "c_inline"]
+private
 val quarter_round:
   st:state ->
   a:idx -> b:idx -> c:idx -> d:idx ->
@@ -212,6 +217,7 @@ let quarter_round st a b c d =
 
 
 [@ "substitute"]
+private
 val column_round:
   st:state ->
   Stack unit
@@ -228,6 +234,7 @@ let column_round st =
 
 
 [@ "substitute"]
+private
 val diagonal_round:
   st:state ->
   Stack unit
@@ -244,6 +251,7 @@ let diagonal_round st =
 
 
 [@ "c_inline"]
+private
 val double_round:
   st:buffer H32.t{length st = 16} ->
   Stack unit
@@ -257,9 +265,10 @@ let double_round st =
     diagonal_round st
 
 
-#reset-options "--initial_fuel 0 --max_fuel 0 --z3rlimit 500"
+#reset-options " --max_fuel 0 --z3rlimit 500"
 
 [@ "c_inline"]
+private
 val rounds:
   st:state ->
   Stack unit
@@ -286,9 +295,10 @@ let rounds st =
   for 0ul 10ul inv f'
 
 
-#reset-options "--initial_fuel 0 --max_fuel 0 --z3rlimit 100"
+#reset-options " --max_fuel 0 --z3rlimit 100"
 
 [@ "c_inline"]
+private
 val sum_states:
   st:state ->
   st':state{disjoint st st'} ->
@@ -303,6 +313,7 @@ let sum_states st st' =
 
 
 [@ "c_inline"]
+private
 val copy_state:
   st:state ->
   st':state{disjoint st st'} ->
@@ -319,13 +330,13 @@ let copy_state st st' =
   Seq.lemma_eq_intro (as_seq h st) (as_seq h st')
 
 
-#reset-options "--initial_fuel 0 --max_fuel 0 --z3rlimit 100"
+#reset-options " --max_fuel 0 --z3rlimit 100"
 
 
 type log_t_ = | MkLog: k:Spec.key -> n:Spec.nonce -> log_t_
 type log_t = Ghost.erased log_t_
 
-
+private
 val lemma_setup_inj:
   k:Spec.key -> n:Spec.nonce -> c:Spec.counter ->
   k':Spec.key -> n':Spec.nonce -> c':Spec.counter -> Lemma
@@ -354,7 +365,8 @@ let invariant (log:log_t) (h:mem) (st:state) : GTot Type0 =
     match log with | MkLog key nonce -> reveal_h32s s == Spec.setup key nonce (H32.v (Seq.index s 12)))
 
 
-private val lemma_invariant:
+private
+val lemma_invariant:
   st:Spec.state ->
   k:Spec.key -> n:Spec.nonce -> c:H32.t -> c':H32.t -> Lemma
     (requires (st == Spec.setup k n (H32.v c)))
@@ -374,15 +386,17 @@ let lemma_invariant s k n c c' =
   Seq.lemma_eq_intro s' (Spec.setup k n (H32.v c'))
 
 
-private val lemma_state_counter:
+private
+val lemma_state_counter:
   k:Spec.key -> n:Spec.nonce -> c:Spec.counter ->
   Lemma (U32.v (Seq.index (Spec.setup k n (c)) 12) == c)
 let lemma_state_counter k n c = ()
 
 
-#reset-options "--max_fuel 0 --max_ifuel 0 --z3rlimit 400"
+#reset-options "--max_fuel 0  --z3rlimit 400"
 
 [@ "c_inline"]
+private
 val chacha20_core:
   log:log_t ->
   k:state ->
@@ -473,19 +487,7 @@ let init st k n =
   Ghost.elift2 (fun (k:uint8_p{length k = 32 /\ live h k}) (n:uint8_p{length n = 12 /\ live h n}) -> MkLog (reveal_sbytes (as_seq h k)) (reveal_sbytes (as_seq h n))) (Ghost.hide k) (Ghost.hide n)
 
 
-#reset-options "--initial_fuel 0 --max_fuel 0 --z3rlimit 100"
-
-(* val lemma_chacha20_counter_mode_1: *)
-(*   ho:mem -> output:uint8_p{live ho output} -> *)
-(*   hi:mem -> input:uint8_p{live hi input} -> *)
-(*   len:U32.t{U32.v len = length output /\ U32.v len = length input /\ U32.v len < 64 /\ U32.v len > 0} -> *)
-(*   k:Spec.key -> n:Spec.nonce -> ctr:U32.t{U32.v ctr + 1 * (length input / 64) < pow2 32} -> Lemma *)
-(*     (Spec.CTR.counter_mode chacha20_ctx chacha20_cipher k n (U32.v ctr) (reveal_sbytes (as_seq hi input)) *)
-(*      == seq_map2 (fun x y -> FStar.UInt8.(x ^^ y)) *)
-(*                              (reveal_sbytes (as_seq hi input)) *)
-(*                              (Seq.slice (Spec.chacha20_block k n (U32.v ctr)) 0 (U32.v len))) *)
-(* #reset-options "--initial_fuel 1 --max_fuel 1 --z3rlimit 100" *)
-(* let lemma_chacha20_counter_mode_1 ho output hi input len k n ctr = () *)
+#reset-options " --max_fuel 0 --z3rlimit 100"
 
 val lemma_chacha20_counter_mode_1:
   ho:mem -> output:uint8_p{live ho output} ->
@@ -512,7 +514,7 @@ let lemma_chacha20_counter_mode_1 ho output hi input len k n ctr =
     Math.Lemmas.lemma_div_le (blocks_len) len ctx.blocklen;
     (* End TODO *)
   let blocks, last_block = Seq.split (as_seq hi input) blocks_len in
-  let cipher_blocks = counter_mode_blocks ctx chacha20_cipher k n counter blocks in
+  let cipher_blocks = counter_mode_blocks ctx chacha20_cipher k n counter (reveal_sbytes blocks) in
   Seq.lemma_eq_intro cipher_blocks Seq.createEmpty;
   assert(ctx.incr * (Seq.length (as_seq hi input) / ctx.blocklen) = 0);
   Seq.lemma_eq_intro (Seq.append Seq.createEmpty (xor #len (reveal_sbytes (as_seq hi input)) (Seq.slice (Spec.chacha20_block k n (UInt32.v ctr)) 0 len))) (xor #len (reveal_sbytes (as_seq hi input)) (Seq.slice (Spec.chacha20_block k n (UInt32.v ctr)) 0 len));
@@ -520,22 +522,7 @@ let lemma_chacha20_counter_mode_1 ho output hi input len k n ctr =
                      (Spec.CTR.xor #(len) (reveal_sbytes (as_seq hi input)) (Seq.slice (Spec.chacha20_block k n (UInt32.v ctr)) 0 (len)))
 
 
-#reset-options "--initial_fuel 0 --max_fuel 0 --z3rlimit 100"
-
-(* val lemma_chacha20_counter_mode_2: *)
-(*   ho:mem -> output:uint8_p{live ho output} -> *)
-(*   hi:mem -> input:uint8_p{live hi input} -> *)
-(*   len:U32.t{U32.v len = length output /\ U32.v len = length input /\ U32.v len >= 64} -> *)
-(*   k:Spec.key -> n:Spec.nonce -> ctr:U32.t{U32.v ctr + (length input / 64) < pow2 32} -> Lemma *)
-(*     (Spec.CTR.counter_mode chacha20_ctx chacha20_cipher k n (U32.v ctr) (reveal_sbytes (as_seq hi input)) *)
-(*      == (let b, plain = Seq.split (reveal_sbytes (as_seq hi input)) 64 in *)
-(*          let mask = Spec.chacha20_block k n (U32.v ctr) in *)
-(*          let eb = seq_map2 (fun x y -> FStar.UInt8.(x ^^ y)) b mask in *)
-(*          let cipher = Spec.CTR.counter_mode chacha20_ctx chacha20_cipher k n (U32.v ctr + 1) plain in *)
-(*          Seq.append eb cipher)) *)
-(* #reset-options "--initial_fuel 1 --max_fuel 1 --z3rlimit 100" *)
-(* let lemma_chacha20_counter_mode_2 ho output hi input len k n ctr = () *)
-
+#reset-options " --max_fuel 0 --z3rlimit 100"
 
 val lemma_chacha20_counter_mode_2:
   ho:mem -> output:uint8_p{live ho output} ->
@@ -549,27 +536,15 @@ val lemma_chacha20_counter_mode_2:
       Math.Lemmas.lemma_mod_plus (Seq.length prefix) 1 (64);
       Math.Lemmas.lemma_div_le (Seq.length prefix) (UInt32.v len) 64;
       Spec.CTR.Lemmas.lemma_div (UInt32.v len) (64);
-    let cipher        = Spec.CTR.counter_mode_blocks chacha20_ctx chacha20_cipher k n (UInt32.v ctr) prefix in
+    let cipher        = Spec.CTR.counter_mode_blocks chacha20_ctx chacha20_cipher k n (UInt32.v ctr) (reveal_sbytes prefix) in
     let mask          = chacha20_cipher k n (UInt32.v ctr + (UInt32.v len / 64 - 1) ) in
-    let eb            = Spec.CTR.xor block mask in
+    let eb            = Spec.CTR.xor (reveal_sbytes block) mask in
     Seq.append cipher eb))
 #reset-options "--initial_fuel 1 --max_fuel 1 --z3rlimit 100"
 let lemma_chacha20_counter_mode_2 ho output hi input len k n ctr = ()
 
 
-#reset-options "--initial_fuel 0 --max_fuel 0 --z3rlimit 100"
-
-(* val lemma_chacha20_counter_mode_0: *)
-(*   ho:mem -> output:uint8_p{live ho output} -> *)
-(*   hi:mem -> input:uint8_p{live hi input} -> *)
-(*   len:U32.t{U32.v len = length output /\ U32.v len = length input /\ U32.v len = 0} -> *)
-(*   k:Spec.key -> n:Spec.nonce -> ctr:U32.t{U32.v ctr + (length input / 64) < pow2 32} -> Lemma *)
-(*     (Spec.CTR.counter_mode chacha20_ctx chacha20_cipher k n (U32.v ctr) (reveal_sbytes (as_seq hi input)) *)
-(*      == reveal_sbytes (as_seq ho output)) *)
-(* #reset-options "--initial_fuel 1 --max_fuel 1 --z3rlimit 100" *)
-(* let lemma_chacha20_counter_mode_0 ho output hi input len k n ctr = *)
-(*   Seq.lemma_eq_intro (as_seq ho output) Seq.createEmpty *)
-
+#reset-options " --max_fuel 0 --z3rlimit 100"
 
 val lemma_chacha20_counter_mode_0:
   ho:mem -> output:uint8_p{live ho output} ->
@@ -584,36 +559,7 @@ let lemma_chacha20_counter_mode_0 ho output hi input len k n ctr =
   Seq.lemma_eq_intro (as_seq ho output) Seq.createEmpty
 
 
-
-
-#reset-options "--initial_fuel 0 --max_fuel 0 --z3rlimit 400"
-
-(* val update_last: *)
-(*   output:uint8_p -> *)
-(*   plain:uint8_p{disjoint output plain} -> *)
-(*   len:U32.t{U32.v len = length output /\ U32.v len = length plain /\ U32.v len < 64 /\ U32.v len > 0} -> *)
-(*   log:log_t -> *)
-(*   st:state{disjoint st output /\ disjoint st plain} -> *)
-(*   ctr:U32.t{U32.v ctr + (length plain / 64) < pow2 32} -> *)
-(*   Stack log_t *)
-(*     (requires (fun h -> live h output /\ live h plain /\ invariant log h st)) *)
-(*     (ensures (fun h0 updated_log h1 -> live h1 output /\ live h0 plain /\ invariant updated_log h1 st *)
-(*       /\ modifies_2 output st h0 h1 *)
-(*       /\ (let o = reveal_sbytes (as_seq h1 output) in *)
-(*          let plain = reveal_sbytes (as_seq h0 plain) in *)
-(*          match Ghost.reveal log with | MkLog k n -> *)
-(*          o == Spec.CTR.counter_mode chacha20_ctx chacha20_cipher k n (U32.v ctr) plain))) *)
-(* let update_last output plain len log st ctr = *)
-(*   let h0 = ST.get() in *)
-(*   push_frame(); *)
-(*   let block = create (uint8_to_sint8 0uy) 64ul in *)
-(*   let l = chacha20_block log block st ctr in *)
-(*   let mask = Buffer.sub block 0ul len in *)
-(*   map2 output plain mask len (fun x y -> H8.(x ^^ y)); *)
-(*   let h1 = ST.get() in *)
-(*   lemma_chacha20_counter_mode_1 h1 output h0 plain len (Ghost.reveal log).k (Ghost.reveal log).n ctr; *)
-(*   pop_frame(); *)
-(*   l *)
+#reset-options " --max_fuel 0 --z3rlimit 400"
 
 val update_last:
   output:uint8_p ->
@@ -678,119 +624,7 @@ let update output plain log st ctr =
   l
 
 
-#reset-options "--initial_fuel 0 --max_fuel 0 --z3rlimit 300"
-
-
-(* val lemma_chacha20_counter_mode: *)
-(*   h0:mem -> h1:mem -> h2:mem -> *)
-(*   output:uint8_p{live h1 output /\ live h2 output /\ live h0 output} -> *)
-(*   plain:uint8_p{live h0 plain /\ live h1 plain /\ live h2 plain} -> *)
-(*   len:UInt32.t{length output = U32.v len /\ length output = length plain /\ U32.v len >= 64} -> *)
-(*   k:Spec.key -> n:Spec.nonce -> ctr:Spec.counter{ctr + U32.v len / 64 < pow2 32} -> *)
-(*   Lemma (requires ( *)
-(*     (let o = reveal_sbytes (as_seq h2 (Buffer.sub output 0ul 64ul)) in *)
-(*      let p = reveal_sbytes (as_seq h0 (Buffer.sub plain 0ul 64ul)) in *)
-(*      let o' = reveal_sbytes (as_seq h2 (Buffer.offset output 64ul)) in *)
-(*      let p' = reveal_sbytes (as_seq h0 (Buffer.offset plain 64ul)) in *)
-(*      o == seq_map2 (fun x y -> FStar.UInt8.(x ^^ y)) p (chacha20_cipher k n (ctr)) *)
-(*      /\ o' == Spec.CTR.counter_mode chacha20_ctx chacha20_cipher k n (ctr + 1) p'))) *)
-(*      (ensures ( *)
-(*        (let o = reveal_sbytes (as_seq h2 output) in *)
-(*         let plain = reveal_sbytes (as_seq h0 plain) in *)
-(*         o == Spec.CTR.counter_mode chacha20_ctx chacha20_cipher k n (ctr) plain))) *)
-(* #reset-options "--initial_fuel 0 --max_fuel 0 --z3rlimit 300" *)
-(* let lemma_chacha20_counter_mode h0 h1 h2 output plain len k n ctr = *)
-(*   cut (ctr + 1 < pow2 32); *)
-(*   Seq.lemma_eq_intro (as_seq h2 (Buffer.sub output 0ul 64ul)) (Seq.slice (as_seq h2 output) 0 64); *)
-(*   Seq.lemma_eq_intro (as_seq h0 (Buffer.sub plain 0ul 64ul)) (Seq.slice (as_seq h0 plain) 0 64); *)
-(*   Seq.lemma_eq_intro (as_seq h2 (Buffer.offset output 64ul)) (Seq.slice (as_seq h2 output) 64 (length output)); *)
-(*   Seq.lemma_eq_intro (as_seq h0 (Buffer.offset plain 64ul)) (Seq.slice (as_seq h0 plain) 64 (length output)); *)
-(*   let b, plainn = Seq.split (reveal_sbytes (as_seq h0 plain)) 64 in *)
-(*   Seq.lemma_eq_intro b (reveal_sbytes (as_seq h0 (Buffer.sub plain 0ul 64ul))); *)
-(*   Seq.lemma_eq_intro plainn (reveal_sbytes (as_seq h0 (Buffer.offset plain 64ul))); *)
-(*   let mask = Spec.chacha20_block k n (ctr) in *)
-(*   let eb = seq_map2 (fun x y -> FStar.UInt8.(x ^^ y)) b mask in *)
-(*   Seq.lemma_eq_intro eb (reveal_sbytes (as_seq h2 (Buffer.sub output 0ul 64ul))); *)
-(*   let cipher = Spec.CTR.counter_mode chacha20_ctx chacha20_cipher k n (ctr + 1) plainn in *)
-(*   Seq.lemma_eq_intro cipher (reveal_sbytes (as_seq h2 (Buffer.offset output 64ul))); *)
-(*   Seq.lemma_eq_intro (Seq.append eb cipher) (reveal_sbytes (as_seq h2 output)); *)
-(*   lemma_chacha20_counter_mode_2 h2 output h0 plain len k n (UInt32.uint_to_t ctr) *)
-
-
-#reset-options "--initial_fuel 0 --max_fuel 0 --z3rlimit 100"
-
-
-(* val chacha20_counter_mode_: *)
-(*   output:uint8_p -> *)
-(*   plain:uint8_p{disjoint output plain} -> *)
-(*   len:U32.t{U32.v len = length output /\ U32.v len = length plain /\ U32.v len < 64} -> *)
-(*   log:log_t -> *)
-(*   st:state{disjoint st output /\ disjoint st plain} -> *)
-(*   ctr:U32.t{U32.v ctr + (length plain / 64) < pow2 32} -> *)
-(*   Stack unit *)
-(*     (requires (fun h -> live h output /\ live h plain /\ invariant log h st)) *)
-(*     (ensures (fun h0 _ h1 -> live h1 output /\ live h0 plain /\ live h1 st *)
-(*       /\ modifies_2 output st h0 h1 *)
-(*       /\ (let o = reveal_sbytes (as_seq h1 output) in *)
-(*          let plain = reveal_sbytes (as_seq h0 plain) in *)
-(*          match Ghost.reveal log with | MkLog k n -> *)
-(*          o == Spec.CTR.counter_mode chacha20_ctx chacha20_cipher k n (U32.v ctr) plain))) *)
-(* let rec chacha20_counter_mode_ output plain len log st ctr = *)
-(*   let h0 = ST.get() in *)
-(*   if U32.(len =^ 0ul) then ( *)
-(*     lemma_chacha20_counter_mode_0 h0 output h0 plain len (Ghost.reveal log).k (Ghost.reveal log).n ctr; *)
-(*     Seq.lemma_eq_intro (as_seq h0 output) Seq.createEmpty *)
-(*   ) else  ( *)
-(*     let _ = update_last output plain len log st ctr in () *)
-(*   ) *)
-
-
-(* #reset-options "--initial_fuel 0 --max_fuel 0 --z3rlimit 100" *)
-
-(* val chacha20_counter_mode: *)
-(*   output:uint8_p -> *)
-(*   plain:uint8_p{disjoint output plain} -> *)
-(*   len:U32.t{U32.v len = length output /\ U32.v len = length plain} -> *)
-(*   log:log_t -> *)
-(*   st:state{disjoint st output /\ disjoint st plain} -> *)
-(*   ctr:U32.t{U32.v ctr + (length plain / 64) < pow2 32} -> *)
-(*   Stack unit *)
-(*     (requires (fun h -> live h output /\ live h plain /\ invariant log h st)) *)
-(*     (ensures (fun h0 _ h1 -> live h1 output /\ live h0 plain /\ live h1 st *)
-(*       /\ modifies_2 output st h0 h1 *)
-(*       /\ (let o = reveal_sbytes (as_seq h1 output) in *)
-(*          let plain = reveal_sbytes (as_seq h0 plain) in *)
-(*          match Ghost.reveal log with | MkLog k n -> *)
-(*          o == Spec.CTR.counter_mode chacha20_ctx chacha20_cipher k n (U32.v ctr) plain))) *)
-(* #reset-options "--initial_fuel 0 --max_fuel 0 --z3rlimit 500" *)
-(* let rec chacha20_counter_mode output plain len log st ctr = *)
-(*   let h0 = ST.get() in *)
-(*   if U32.(len <^ 64ul) then chacha20_counter_mode_ output plain len log st ctr *)
-(*   else ( *)
-(*     let b  = Buffer.sub plain 0ul 64ul in *)
-(*     let b' = Buffer.offset plain 64ul in *)
-(*     let o  = Buffer.sub output 0ul 64ul in *)
-(*     let o' = Buffer.offset output 64ul in *)
-(*     let log' = update o b log st ctr in *)
-(*     let h = ST.get() in *)
-(*     let l = chacha20_counter_mode o' b' U32.(len -^ 64ul) log st U32.(ctr +^ 1ul) in *)
-(*     let h' = ST.get() in *)
-(*     cut (let o' = reveal_sbytes (as_seq h' o') in *)
-(*          let b' = reveal_sbytes (as_seq h b')  in *)
-(*          o' == Spec.CTR.counter_mode chacha20_ctx chacha20_cipher *)
-(*                                                (Ghost.reveal log).k (Ghost.reveal log).n *)
-(*                                                (U32.v ctr + 1) (b')); *)
-(*     no_upd_lemma_2 h0 h o st b; *)
-(*     no_upd_lemma_2 h0 h o st b'; *)
-(*     no_upd_lemma_2 h0 h o st o'; *)
-(*     no_upd_lemma_2 h h' o' st b; *)
-(*     no_upd_lemma_2 h h' o'  st b'; *)
-(*     no_upd_lemma_2 h h' o' st o; *)
-(*     lemma_chacha20_counter_mode h0 h h' output plain len (Ghost.reveal log).k (Ghost.reveal log).n (U32.v ctr) *)
-(*   ) *)
-
-
-#reset-options "--max_fuel 0 --max_ifuel 0 --z3rlimit 100"
+#reset-options " --max_fuel 0 --z3rlimit 100"
 
 private
 val lemma_aux_modifies_2: #a:Type -> #a':Type -> h:mem -> b:buffer a{live h b} -> b':buffer a'{live h b'} -> Lemma
@@ -811,7 +645,7 @@ let lemma_chacha20_counter_mode_def_0 s k n ctr =
   Seq.lemma_eq_intro s Seq.createEmpty
 
 
-#reset-options "--max_fuel 0 --max_ifuel 0 --z3rlimit 200"
+#reset-options "--max_fuel 0  --z3rlimit 200"
 
 private
 val chacha20_counter_mode_blocks:
@@ -836,7 +670,7 @@ let rec chacha20_counter_mode_blocks output plain len log st ctr =
     live h1 output /\ invariant log h1 st /\ modifies_2 output st h0 h1 /\ 0 <= i /\ i <= UInt32.v len
     /\ (match Ghost.reveal log with | MkLog k n ->
       reveal_sbytes (Seq.slice (as_seq h1 output) 0 (64 * i))
-      == Spec.CTR.counter_mode_blocks chacha20_ctx chacha20_cipher k n (UInt32.v ctr) (Seq.slice (as_seq h0 plain) 0 (64 * i)))
+      == Spec.CTR.counter_mode_blocks chacha20_ctx chacha20_cipher k n (UInt32.v ctr) (reveal_sbytes (Seq.slice (as_seq h0 plain) 0 (64 * i))))
   in
   let f' (i:UInt32.t{ FStar.UInt32.( 0 <= v i /\ v i < v len ) }): Stack unit
     (requires (fun h -> inv h (UInt32.v i)))
@@ -876,7 +710,6 @@ let rec chacha20_counter_mode_blocks output plain len log st ctr =
   let i0 = Buffer.sub plain  0ul 0ul in
   Seq.lemma_eq_intro (as_seq h0 o0) (Seq.slice (as_seq h0 output) 0 0);
   Seq.lemma_eq_intro (as_seq h0 i0) (Seq.slice (as_seq h0 plain) 0 0);
-  (* lemma_chacha20_counter_mode_0 h0 o0 h0 i0 0ul (Ghost.reveal log).k (Ghost.reveal log).n ctr; *)
   lemma_aux_modifies_2 h0 output st;
   lemma_chacha20_counter_mode_def_0 (Seq.slice (as_seq h0 plain) 0 0) (Ghost.reveal log).k (Ghost.reveal log).n ctr;
   Seq.lemma_eq_intro (Seq.slice (as_seq h0 plain) 0 0) Seq.createEmpty;
@@ -924,11 +757,11 @@ let chacha20_counter_mode output plain len log st ctr =
   Seq.lemma_eq_intro (Seq.append (as_seq h output') Seq.createEmpty) (as_seq h output');
   Seq.lemma_eq_intro (as_seq h output) (Seq.append (as_seq h output') (as_seq h output''));
   Seq.lemma_eq_intro (as_seq h0 plain) (Seq.append (as_seq h0 plain') (as_seq h0 plain''));
-  Seq.lemma_eq_intro (as_seq h output) (Spec.CTR.counter_mode chacha20_ctx chacha20_cipher (Ghost.reveal log).k (Ghost.reveal log).n (UInt32.v ctr) (as_seq h0 plain));
+  Seq.lemma_eq_intro (reveal_sbytes (as_seq h output)) (Spec.CTR.counter_mode chacha20_ctx chacha20_cipher (Ghost.reveal log).k (Ghost.reveal log).n (UInt32.v ctr) (reveal_sbytes (as_seq h0 plain)));
   ()
 
 
-#reset-options "--initial_fuel 0 --max_fuel 0 --z3rlimit 20"
+#reset-options "--max_fuel 0 --z3rlimit 20"
 
 val chacha20:
   output:uint8_p ->
